proof: refinement

policy_proof/coq/security.v
@@ -3,20 +3,44 @@ Require Import Unicode.Utf8.
 
 Require Import query.
 Require Import types.
+Require Import relation.
+Require Import data_model.
 
-(* todo *)
-Fixpoint env_ok s (e : ℰ s) : Prop :=
+Definition policy_ok_tuple: ∀ s (Γ: Policy.context), Tuple.tuple s -> Prop.
+refine (
+  fix policy_ok_tuple' s (Γ: Policy.context): Tuple.tuple s -> Prop :=
+    match s as s' return s = s' -> Tuple.tuple s' -> Prop with 
+    | nil => fun _ _ => True
+    | bt :: t' => fun _ _ => _
+    end (eq_refl _)
+).
+  destruct t.
+  pose (Policy.label_lookup (snd p) Γ).
+  destruct o.
+  - exact (Policy.can_release p0 ∧ policy_ok_tuple' _ Γ t).
+  - exact False.
+Defined.
+  
+Fixpoint policy_ok_relation s (Γ: Policy.context) (r: relation s) : Prop :=
+  match r with
+    | nil => True
+    | t :: r' => policy_ok_tuple _ Γ t ∧ policy_ok_relation _ Γ r'
+  end.
+
+Definition policy_ok s (Γ: Policy.context) (e : ℰ s) : Prop :=
   match e with
     | nil => True
-    | (x, t) :: e' =>  False ∨ env_ok _ e'
+    | es :: _ =>
+        match es with (r, _, _, _) => policy_ok_relation _ Γ r end
   end.
 
 (* todo *)
 Theorem secure_query:
   ∀ s s' Γ Γ' β β' e e' o c,
-    config_ok s Γ β e =[ o ]=> c →
+    ⟨ s Γ β e ⟩ =[ o ]=> c →
       c = config_error ∨
-      c = config_ok s' Γ' β' e' ∧ env_ok s' e'.
+      c = ⟨ s' Γ' β' e' ⟩ ∧ policy_ok s' Γ' e'.
 Proof.
-  intros.
+  intros. induction H; simpl in *.
+  - right. split.
 Admitted.
